compiler/backend/reg_alloc/proofs/linear_scanProofScript.sml
@@ -15,65 +15,6 @@ val _ = temp_overload_on ("return", ``st_ex_return``);
 
 val _ = hide "state";
 
-val is_subset_compute_eq = Q.store_thm("is_subset_compute_eq",
-    `!s1 s2. is_subset_compute s1 s2 <=>
-    !x. (?y1. lookup x s1 = SOME y1) ==> (?y2. lookup x s2 = SOME y2)`,
-    rpt strip_tac >>
-    eq_tac THEN1 (
-      rw [is_subset_compute_def] >>
-      `MEM (x, y1) (toAList s1)` by metis_tac [MEM_toAList] >>
-      `(\(a, b). lookup a s2 <> NONE) (x, y1)` by fs [EVERY_MEM] >>
-      fs [] >>
-      Cases_on `lookup x s2` >> fs[]
-    ) >>
-    rw [is_subset_compute_def] >>
-    `!x. (?y1. MEM (x, y1) (toAList s1)) ==> (?y2. lookup x s2 = SOME y2)` by fs [MEM_toAList] >>
-    pop_assum mp_tac >>
-    qspec_tac (`toAList s1`, `l`) >>
-    Induct_on `l` >>
-    rw [] >>
-    fs [PULL_EXISTS] >>
-    Cases_on `h` >>
-    rw [] >>
-    pop_assum (qspecl_then [`q`,`r`] assume_tac) >>
-    Cases_on `lookup q s2` >> rw []
-)
-
-val is_subset_eq = Q.store_thm("is_subset_eq",
-    `!s1 s2. is_subset s1 s2 <=>
-    !x. (?y1. lookup x s1 = SOME y1) ==> (?y2. lookup x s2 = SOME y2)`,
-    rw [] >>
-    eq_tac THEN1 (
-        rw [is_subset_def] >>
-        `x IN (domain s1)` by simp [domain_lookup] >>
-        `x IN (domain s2)` by fs [SUBSET_DEF] >>
-        fs [domain_lookup]
-    ) >>
-    fs [PULL_EXISTS] >>
-    rw [is_subset_def, SUBSET_DEF] >>
-    `?y1. lookup x s1 = SOME y1` by fs [domain_lookup] >>
-    `?y2. lookup x s2 = SOME y2` by simp [] >>
-    fs [domain_lookup]
-)
-
-val union_monotone = Q.store_thm("union_monotone",
-    `!s1 s2 s1' s2'.
-    is_subset s1 s1' /\ is_subset s2 s2' ==> is_subset (union s1 s2) (union s1' s2')`,
-    rpt strip_tac >>
-    fs [is_subset_eq, lookup_union, PULL_EXISTS] >>
-    rpt gen_tac >>
-    NTAC 2 (first_x_assum (qspecl_then [`x`, `y1`] assume_tac)) >>
-    Cases_on `lookup x s1` >> Cases_on `lookup x s1'` >> rw []
-)
-
-val insert_monotone = Q.store_thm("insert_monotone",
-    `!s1 s2 x v.
-    is_subset s1 s2 ==> is_subset (insert x a s1) (insert x a s2)`,
-    rw [is_subset_eq, lookup_insert] >>
-    Cases_on `x' = x` >>
-    rw [] >> metis_tac []
-)
-
 val numset_list_insert_FOLDL = Q.store_thm("numset_list_insert_FOLDL",
     `!l live. numset_list_insert l live = FOLDL (\live x. insert x () live) live l`,
     Induct_on `l` >> rw [numset_list_insert_def]
@@ -89,15 +30,6 @@ val both_numset_list_insert_equal = Q.store_thm("both_numset_list_insert_equal",
     numset_list_insert l live = numset_list_insert_nottailrec (REVERSE l) live`,
 
     rw [numset_list_insert_FOLDL, numset_list_insert_nottailrec_FOLDR, FOLDR_FOLDL_REVERSE]
-)
-
-val numset_list_insert_monotone = Q.store_thm("numset_list_insert_monotone",
-    `!l s1 s2.
-    is_subset s1 s2 ==> is_subset (numset_list_insert l s1) (numset_list_insert l s2)`,
-    Induct_on `l` >>
-    rw [numset_list_insert_def] >>
-    `is_subset (insert h () s1) (insert h () s2)` by simp [insert_monotone] >>
-    rw []
 )
 
 val domain_numset_list_insert = Q.store_thm("domain_numset_list_insert",
@@ -148,222 +80,17 @@ val numset_list_insert_FILTER = Q.store_thm("numset_list_insert_FILTER",
     ) >>
     rw [both_numset_list_insert_equal, GSYM FILTER_REVERSE] >>
     qabbrev_tac `l' = REVERSE l` >>
-    WEAKEN_TAC (fn x => true) >>
+    qpat_x_assum `Abbrev _` kall_tac >>
     Induct_on `l'` >>
     rw [numset_list_insert_nottailrec_def] >>
     Cases_on `lookup h live` >> fs [NOT_SOME_NONE] >>
     simp [lookup_insert_id]
 )
 
-
-val delete_monotone = Q.store_thm("delete_monotone",
-    `!s1 s2 x v.
-    is_subset s1 s2 ==> is_subset (delete x s1) (delete x s2)`,
-    rw [is_subset_eq, lookup_delete, IS_SOME_EXISTS] >> metis_tac [NOT_SOME_NONE]
-)
-
-val numset_list_delete_monotone = Q.store_thm("numset_list_delete_monotone",
-    `!l s1 s2.
-    is_subset s1 s2 ==> is_subset (numset_list_delete l s1) (numset_list_delete l s2)`,
-    Induct_on `l` >>
-    rw [numset_list_delete_def] >>
-    `is_subset (delete h s1) (delete h s2)` by simp [delete_monotone] >>
-    rw []
-)
-
 val domain_numset_list_delete = Q.store_thm("domain_numset_list_delete",
     `!l s.  domain (numset_list_delete l s) = (domain s) DIFF (set l)`,
     Induct_on `l` >>
     rw [numset_list_delete_def, DIFF_INSERT]
-)
-
-val check_partial_col_input_monotone = Q.store_thm("check_partial_col_input_monotone",
-    `!f live1 flive1 live2 flive2 l liveout2 fliveout2.
-    IMAGE f (domain live1) = domain flive1 /\ IMAGE f (domain live2) = domain flive2 ==>
-    is_subset live1 live2 ==>
-    INJ f (domain live2) UNIV ==>
-    check_partial_col f l live2 flive2 = SOME (liveout2, fliveout2) ==>
-    ?liveout1 fliveout1. check_partial_col f l live1 flive1 = SOME (liveout1, fliveout1)
-    `,
-
-    sg `!x f s fs. (domain fs) = (IMAGE f (domain s)) /\ lookup x s = SOME () ==> lookup (f x) fs = SOME ()` THEN1 (
-        rw [] >>
-        `x IN (domain s)` by fs [domain_lookup] >>
-        `f x IN (IMAGE f (domain s))` by fs [IMAGE_IN] >>
-        `f x IN (domain fs)` by metis_tac [] >>
-        fs [domain_lookup]
-    ) >>
-
-    Induct_on `l` >>
-    rw [check_partial_col_def] >>
-
-    `!x. lookup x live1 = SOME () ==> lookup (f x) flive1 = SOME ()` by metis_tac [] >>
-    `!x. lookup x live2 = SOME () ==> lookup (f x) flive2 = SOME ()` by metis_tac [] >>
-
-    sg `!x. ((?y. lookup x flive1 = SOME y) /\ lookup x flive2 = NONE) ==> F` THEN1 (
-        rpt strip_tac >>
-        fs [is_subset_def] >>
-        `(IMAGE f (domain live1)) SUBSET (IMAGE f (domain live2))` by fs [IMAGE_SUBSET] >>
-        `(domain flive1) SUBSET (domain flive2)` by metis_tac [] >>
-        `x IN (domain flive1)` by fs [domain_lookup] >>
-        `x IN (domain flive2)` by fs [SUBSET_DEF] >>
-        `?y. lookup x flive2 = SOME y` by fs [domain_lookup] >>
-        fs [NOT_SOME_NONE]
-    ) >>
-
-    Cases_on `lookup h live1` >>
-    Cases_on `lookup h live2` >>
-    rw []
-
-    (* NONE NONE *)
-    THEN1 (
-        Cases_on `lookup (f h) flive1` >>
-        Cases_on `lookup (f h) flive2` >>
-        fs []
-        (* NONE NONE *)
-        THEN1 (
-          `IMAGE f (domain (insert h () live2)) = domain (insert (f h) () flive2)` by rw [domain_insert, IMAGE_INSERT] >>
-          `IMAGE f (domain (insert h () live1)) = domain (insert (f h) () flive1)` by rw [domain_insert, IMAGE_INSERT] >>
-          sg `INJ f (domain (insert h () live2)) UNIV` THEN1 (
-            rw [domain_insert, INJ_INSERT] >>
-            `(f y) IN (IMAGE f (domain live2))` by fs [IMAGE_IN] >>
-            `(f y) IN (domain flive2)` by metis_tac [] >>
-            `(f h) IN (domain flive2)` by metis_tac [] >>
-            `?y. lookup (f h) flive2 = SOME y` by fs [domain_lookup] >>
-            fs [NOT_SOME_NONE]
-          ) >>
-          `is_subset (insert h () live1) (insert h () live2)` by rw [insert_monotone] >>
-          first_x_assum drule >>
-          metis_tac []
-        )
-        (* SOME NONE *)
-        THEN1 (
-            metis_tac []
-        )
-    )
-    (* NONE SOME *)
-    THEN1 (
-        Cases_on `lookup (f h) flive2` >> fs [] THEN1 (
-            (* Contradiction *)
-            `lookup (f h) flive2 = SOME ()` by rfs [] >>
-            metis_tac [NOT_SOME_NONE]
-        ) >>
-        Cases_on `lookup (f h) flive1` >> fs [] THEN1 (
-            `IMAGE f (domain (insert h () live1)) = domain (insert (f h) () flive1)` by rw [domain_insert, IMAGE_INSERT] >>
-            sg `is_subset (insert h () live1) live2` THEN1 (
-                rw [is_subset_eq, lookup_insert] >>
-                Cases_on `x = h` >> fs [is_subset_eq]
-            ) >>
-            first_x_assum (qspecl_then [`f`, `insert h () live1`, `insert (f h) () flive1`] assume_tac) >>
-            metis_tac [] (* slow :( *)
-        ) >>
-        sg `?x.f h = f x /\ x IN (domain live1)` THEN1 (
-            `(f h) IN (domain flive1)` by fs [domain_lookup] >>
-            `(f h) IN (IMAGE f (domain live1))` by metis_tac [] >>
-            metis_tac [IMAGE_applied, IN_DEF]
-        ) >>
-        `lookup h live1 <> SOME ()` by rw [NOT_SOME_NONE] >>
-        `~(h IN (domain live1))` by rw [domain_lookup] >>
-        `x <> h` by metis_tac [] >>
-        `x IN (domain live2)` by fs [is_subset_def, SUBSET_DEF] >>
-        `h IN (domain live2)` by fs [domain_lookup] >>
-        metis_tac [INJ_DEF]
-    )
-    (* SOME NONE *)
-    THEN1 (
-        `h IN (domain live1)` by fs [domain_lookup] >>
-        `h IN (domain live2)` by fs [SUBSET_DEF, is_subset_def] >>
-        `lookup h live2 = SOME ()` by fs [domain_lookup] >>
-        metis_tac [NOT_SOME_NONE]
-    )
-    (* SOME SOME *)
-    THEN1 (
-        fs [] >>
-        `lookup (f h) flive1 = SOME ()` by rfs [] >>
-        `lookup (f h) flive2 = SOME ()` by rfs [] >>
-        metis_tac []
-    )
-)
-
-val numset_list_delete_IMAGE = Q.store_thm("numset_list_delete_IMAGE",
-    `!f l live flive a b.
-    domain flive = IMAGE f (domain live) ==>
-    INJ f (domain live) UNIV ==>
-    check_partial_col f l live flive = SOME(a, b) ==>
-    domain (numset_list_delete (MAP f l) flive) = IMAGE f (domain (numset_list_delete l live))`,
-
-    Induct_on `l` >>
-    rw [numset_list_delete_def, check_partial_col_def] >> rw [] >>
-    Cases_on `lookup h live` >> fs [] THEN1 (
-        Cases_on `lookup (f h) flive` >> fs [] >>
-        `h NOTIN domain live` by fs [lookup_NONE_domain] >>
-        `(f h) NOTIN domain flive` by fs [lookup_NONE_domain] >>
-        `(f h) NOTIN (IMAGE f (domain live))` by metis_tac [] >>
-        `domain (delete (f h) flive) = IMAGE f (domain (delete h live))` by rw [domain_delete, DELETE_NON_ELEMENT_RWT] >>
-        `domain (insert (f h) () flive) = IMAGE f (domain (insert h () live))` by rw [domain_insert] >>
-        `(domain live DELETE h) SUBSET domain live` by rw [DELETE_SUBSET] >>
-        `INJ f (domain (delete h live)) UNIV` by metis_tac [domain_delete, INJ_SUBSET, UNIV_SUBSET] >>
-        sg `INJ f (domain (insert h () live)) UNIV` THEN1 (
-            rw [domain_insert, INJ_INSERT] >>
-            `f y IN IMAGE f (domain live)` by rw [IMAGE_IN] >>
-            metis_tac []
-        ) >>
-        `is_subset (delete h live) live` by rw [is_subset_def, domain_delete, DELETE_SUBSET] >>
-        `is_subset live (insert h () live)` by rw [is_subset_def, domain_insert, INSERT_SUBSET] >>
-        `?a b. check_partial_col f l live flive = SOME (a, b)` by metis_tac [check_partial_col_input_monotone] >>
-        `?a b. check_partial_col f l (delete h live) (delete (f h) flive) = SOME (a, b)` by metis_tac [check_partial_col_input_monotone] >>
-        rw []
-    ) >>
-
-    `h IN domain live` by rw [domain_lookup] >>
-    `f h IN domain flive` by rw [IMAGE_IN] >>
-    sg `domain (delete (f h) flive) = IMAGE f (domain (delete h live))` THEN1 (
-      rw [domain_delete] >> rw [EXTENSION] >>
-      eq_tac THEN1 (
-        rw [] >> qexists_tac `x'` >> simp [] >> CCONTR_TAC >> fs []
-      ) >>
-      rw [] THEN1 (
-        qexists_tac `x'` >> simp []
-      ) >>
-      CCONTR_TAC >> fs [] >> `x' = h` by metis_tac [INJ_DEF]
-    ) >>
-    `domain (delete h live) SUBSET domain live` by rw [domain_delete, SUBSET_DELETE] >>
-    `INJ f (domain (delete h live)) UNIV` by metis_tac [INJ_SUBSET, UNIV_SUBSET] >>
-    `?a b. check_partial_col f l live flive = SOME (a, b)` by metis_tac [check_partial_col_input_monotone, is_subset_def] >>
-    `?a b. check_partial_col f l (delete h live) (delete (f h) flive) = SOME (a, b)` by metis_tac [check_partial_col_input_monotone, is_subset_def] >>
-    rw []
-)
-
-val check_partial_col_output_monotone = Q.store_thm("check_partial_col_output_monotone",
-    `!f live1 flive1 live2 flive2 l liveout2 fliveout2.
-    is_subset live1 live2 ==>
-    check_partial_col f l live1 flive1 = SOME (liveout1, fliveout1) ==>
-    check_partial_col f l live2 flive2 = SOME (liveout2, fliveout2) ==>
-    is_subset liveout1 liveout2
-    `,
-    rw [is_subset_def] >>
-    (*`domain liveout1 = (set l) UNION (domain live1)` by metis_tac [check_partial_col_domain, FST]*)
-    `domain liveout1 = (set l) UNION (domain live1)` by metis_tac [check_partial_col_domain, FST] >>
-    `domain liveout2 = (set l) UNION (domain live2)` by metis_tac [check_partial_col_domain, FST] >>
-    `(domain live2) SUBSET ((set l) UNION (domain live2))` by rw [SUBSET_UNION] >>
-    rw [] >>
-    metis_tac [SUBSET_TRANS]
-)
-
-val check_partial_col_IMAGE = Q.store_thm("check_partial_col_IMAGE",`
-    !f l live flive live' flive'.
-    (domain flive) = IMAGE f (domain live) ==>
-    check_partial_col f l live flive = SOME (live', flive') ==>
-    (domain flive') = IMAGE f (domain live')
-    `,
-
-    Induct_on `l` >>
-    fs [check_partial_col_def] >> rw [] >>
-    Cases_on`lookup h live` >>
-    Cases_on`lookup (f h) flive` >>
-    fs [] >>
-    `domain (insert (f h) () flive) = IMAGE f (domain (insert h () live))` by rw [domain_insert] >>
-    metis_tac []
 )
 
 val check_partial_col_success_INJ_lemma = Q.prove(`
@@ -401,11 +128,69 @@ val check_partial_col_success_INJ = Q.store_thm("check_partial_col_success_INJ",
     INJ f (domain live) UNIV /\
     check_partial_col f l live flive = SOME (live',flive')
     ==>
+    INJ f (set l UNION domain live) UNIV /\
     INJ f (domain live') UNIV`,
 
     rw [] >>
     `domain live' = set l UNION domain live` by metis_tac [check_partial_col_domain, FST] >>
     metis_tac [check_partial_col_success_INJ_lemma]
+)
+
+val check_partial_col_input_monotone = Q.store_thm("check_partial_col_input_monotone",
+    `!f live1 flive1 live2 flive2 l v.
+    IMAGE f (domain live1) = domain flive1 /\ IMAGE f (domain live2) = domain flive2 ==>
+    domain live1 SUBSET domain live2 ==>
+    INJ f (domain live2) UNIV ==>
+    check_partial_col f l live2 flive2 = SOME v ==>
+    ?livein1 flivein1. check_partial_col f l live1 flive1 = SOME (livein1, flivein1)
+    `,
+
+    rw [] >>
+    PairCases_on `v` >>
+    `INJ f (set l UNION domain live2) UNIV` by metis_tac [check_partial_col_success_INJ] >>
+    `set l UNION domain live1 SUBSET set l UNION domain live2` by fs [SUBSET_DEF] >>
+    `INJ f (set l UNION domain live1) UNIV` by metis_tac [INJ_SUBSET, UNIV_SUBSET] >>
+    metis_tac [check_partial_col_success]
+)
+
+val numset_list_delete_IMAGE = Q.store_thm("numset_list_delete_IMAGE",
+    `!f l live flive v.
+    domain flive = IMAGE f (domain live) ==>
+    INJ f (domain live) UNIV ==>
+    check_partial_col f l live flive = SOME v ==>
+    domain (numset_list_delete (MAP f l) flive) = IMAGE f (domain (numset_list_delete l live))`,
+
+    rw [] >>
+    PairCases_on `v` >>
+    `INJ f (set l UNION domain live) UNIV` by metis_tac [check_partial_col_success_INJ] >>
+    rw [domain_numset_list_delete, EXTENSION] >>
+    eq_tac >> strip_tac
+    THEN1 (
+        fs [MEM_MAP] >>
+        metis_tac []
+    )
+    THEN1 (
+        strip_tac
+        THEN1 metis_tac [] >>
+        CCONTR_TAC >> fs [MEM_MAP, INJ_IFF] >>
+        metis_tac []
+    )
+)
+
+val check_partial_col_IMAGE = Q.store_thm("check_partial_col_IMAGE",`
+    !f l live flive live' flive'.
+    (domain flive) = IMAGE f (domain live) ==>
+    check_partial_col f l live flive = SOME (live', flive') ==>
+    (domain flive') = IMAGE f (domain live')
+    `,
+
+    Induct_on `l` >>
+    fs [check_partial_col_def] >> rw [] >>
+    Cases_on`lookup h live` >>
+    Cases_on`lookup (f h) flive` >>
+    fs [] >>
+    `domain (insert (f h) () flive) = IMAGE f (domain (insert h () live))` by rw [domain_insert] >>
+    metis_tac []
 )
 
 val branch_domain = Q.store_thm("branch_domain",`
@@ -443,7 +228,7 @@ val check_partial_col_list_monotone = Q.store_thm("check_partial_col_list_monoto
     `!f live flive (s1 : num_set) (s2 : num_set) a b.
     domain flive = IMAGE f (domain live) ==>
     INJ f (domain live) UNIV ==>
-    is_subset s1 s2 ==>
+    domain s1 SUBSET domain s2 ==>
     check_partial_col f (MAP FST (toAList s2)) live flive= SOME (a, b) ==>
     ?c d. check_partial_col f (MAP FST (toAList s1)) live flive = SOME (c, d)`,
 
@@ -451,7 +236,7 @@ val check_partial_col_list_monotone = Q.store_thm("check_partial_col_list_monoto
     `!(s : num_set). set (MAP FST (toAList s)) = domain s` by rw [EXTENSION, MEM_MAP, MEM_toAList, EXISTS_PROD, domain_lookup] >>
     `INJ f (domain a) UNIV` by metis_tac [check_partial_col_success_INJ] >>
     `domain a = (domain s2 UNION domain live)` by metis_tac [check_partial_col_domain, FST] >>
-    `domain s1 UNION domain live SUBSET domain a` by fs [is_subset_def, SUBSET_DEF] >>
+    `domain s1 UNION domain live SUBSET domain a` by fs [SUBSET_DEF] >>
     `INJ f (domain s1 UNION domain live) UNIV` by metis_tac [INJ_SUBSET, UNIV_SUBSET] >>
     metis_tac [check_partial_col_success]
 )
@@ -469,8 +254,7 @@ val check_live_tree_success = Q.store_thm("check_live_tree_success", `
     (* Writes *)
     THEN1 (
       rw [check_live_tree_def] >>
-      Cases_on `check_partial_col f l live flive` >> fs [] >>
-      Cases_on `x`
+      fs [case_eq_thms]
       THEN1 (
         metis_tac [numset_list_delete_IMAGE]
       )
@@ -482,42 +266,29 @@ val check_live_tree_success = Q.store_thm("check_live_tree_success", `
     (* Reads *)
     THEN1 (
       rw [check_live_tree_def]
-      THEN1 (
-        metis_tac [check_partial_col_IMAGE]
-      )
-      THEN1 (
-        metis_tac [check_partial_col_success_INJ]
-      )
+      THEN1 metis_tac [check_partial_col_IMAGE]
+      THEN1 metis_tac [check_partial_col_success_INJ]
     )
     (* Branch *)
     THEN1 (
       rw [check_live_tree_def] >>
-      Cases_on `check_live_tree f lt live flive` >> fs [] >>
-      Cases_on `x` >> fs [] >>
-      Cases_on `check_live_tree f lt' live flive` >> fs [] >>
-      Cases_on `x` >> fs []
+      fs [case_eq_thms] >> rveq
       THEN1 (
         metis_tac [check_partial_col_IMAGE]
       )
       THEN1 (
-        `INJ f (domain q) UNIV` by metis_tac [] >>
-        `domain r = IMAGE f (domain q)` by metis_tac [check_partial_col_IMAGE] >>
+        `INJ f (domain livein1) UNIV` by metis_tac [] >>
+        `domain flivein1 = IMAGE f (domain livein1)` by metis_tac [check_partial_col_IMAGE] >>
         metis_tac [check_partial_col_success_INJ]
       )
     )
     (* Seq *)
     THEN1 (
       rw [check_live_tree_def] >>
-      Cases_on `check_live_tree f lt' live flive` >> fs [] >>
-      Cases_on `x` >> fs [] >>
-      `domain r = IMAGE f (domain q)` by metis_tac []
-      THEN1 (
-        metis_tac []
-      )
-      THEN1 (
-        `INJ f (domain q) UNIV` by metis_tac [] >>
-        metis_tac []
-      )
+      fs [case_eq_thms] >> rveq >>
+      `domain flivein2 = IMAGE f (domain livein2)` by metis_tac [] >>
+      `INJ f (domain livein2) UNIV` by metis_tac [] >>
+      metis_tac []
     )
 )
 
@@ -560,12 +331,12 @@ val check_col_success = Q.store_thm("check_col_success",
 )
 
 val check_clash_tree_output = Q.store_thm("check_clash_tree_output", `
-    !f ct live flive live' flive'.
+    !f ct live flive livein flivein.
     domain flive = IMAGE f (domain live) /\
     INJ f (domain live) UNIV /\
-    check_clash_tree f ct live flive = SOME (live', flive') ==>
-    domain flive' = IMAGE f (domain live') /\
-    INJ f (domain live') UNIV`,
+    check_clash_tree f ct live flive = SOME (livein, flivein) ==>
+    domain flivein = IMAGE f (domain livein) /\
+    INJ f (domain livein) UNIV`,
 
     Induct_on `ct` >>
     simp [check_clash_tree_def]
@@ -573,8 +344,7 @@ val check_clash_tree_output = Q.store_thm("check_clash_tree_output", `
     (* Delta *)
     THEN1 (
       rpt gen_tac >> strip_tac >>
-      Cases_on `check_partial_col f l live flive` >> fs [] >>
-      Cases_on `x` >> fs [] >>
+      fs [case_eq_thms] >>
       `domain (numset_list_delete (MAP f l) flive) = IMAGE f (domain (numset_list_delete l live))` by metis_tac [numset_list_delete_IMAGE] >>
       `domain (numset_list_delete l live) SUBSET (domain live)` by rw [domain_numset_list_delete] >>
       `INJ f (domain (numset_list_delete l live)) UNIV` by metis_tac [INJ_SUBSET, UNIV_SUBSET] >>
@@ -589,39 +359,34 @@ val check_clash_tree_output = Q.store_thm("check_clash_tree_output", `
     (* Branch *)
     THEN1 (
         rpt gen_tac >> strip_tac >>
-        Cases_on `check_clash_tree f ct live flive` >> fs [] >>
-        Cases_on `x` >> fs [] >>
-        Cases_on `check_clash_tree f ct' live flive` >> fs [] >>
-        Cases_on `x` >> fs [] >>
-        Cases_on `o'` >> fs [] THEN1 (
-            `domain r = IMAGE f (domain q)` by metis_tac [check_partial_col_IMAGE] >>
-            `INJ f (domain q) UNIV` by metis_tac [check_partial_col_success_INJ] >>
+        fs [case_eq_thms] >> rveq
+        THEN1 (
+            `domain ft1_out = IMAGE f (domain t1_out)` by metis_tac [check_partial_col_IMAGE] >>
+            `INJ f (domain t1_out) UNIV` by metis_tac [check_partial_col_success_INJ] >>
             strip_tac
             THEN1 metis_tac [check_partial_col_IMAGE]
             THEN1 metis_tac [check_partial_col_success_INJ]
 
-        ) >>
-        metis_tac [check_col_output]
+        )
+        THEN1 metis_tac [check_col_output]
     )
     (* Seq *)
     THEN1 (
         rpt gen_tac >> strip_tac >>
-        Cases_on `check_clash_tree f ct' live flive` >> fs [] >>
-        Cases_on `x` >> fs [] >>
-        `domain r = IMAGE f (domain q) /\ INJ f (domain q) UNIV` by metis_tac [] >>
+        fs [case_eq_thms] >> rveq >>
+        `domain ft2_out = IMAGE f (domain t2_out) /\ INJ f (domain t2_out) UNIV` by metis_tac [] >>
         metis_tac []
     )
 )
 
 val get_live_tree_correct_lemma = Q.store_thm("get_live_tree_correct_lemma",
-    `!f live1 flive1 live2 flive2 ct live2' flive2'.
-    IMAGE f (domain live1) = domain flive1 /\ IMAGE f (domain live2) = domain flive2 ==>
-    INJ f (domain live2) UNIV ==>
-    is_subset live1 live2 ==>
-    check_live_tree f (get_live_tree ct) live2 flive2 = SOME (live2', flive2') ==>
-    ?live1' flive1'. check_clash_tree f ct live1 flive1 = SOME (live1', flive1') /\
-    IMAGE f (domain live1') = domain flive1' /\
-    is_subset live1' live2'
+    `!f live flive live' flive' ct livein' flivein'.
+    IMAGE f (domain live) = domain flive /\ IMAGE f (domain live') = domain flive' ==>
+    INJ f (domain live') UNIV ==>
+    domain live SUBSET domain live' ==>
+    check_live_tree f (get_live_tree ct) live' flive' = SOME (livein', flivein') ==>
+    ?livein flivein. check_clash_tree f ct live flive = SOME (livein, flivein) /\
+    domain livein SUBSET domain livein'
     `,
 
     Induct_on `ct`
@@ -629,145 +394,112 @@ val get_live_tree_correct_lemma = Q.store_thm("get_live_tree_correct_lemma",
     (* Delta *)
     THEN1 (
         rw [check_clash_tree_def, get_live_tree_def, check_live_tree_def] >>
-        fs [check_live_tree_def] >>
-        Cases_on `check_partial_col f l live2 flive2` >> fs [] >>
-        Cases_on `x` >>
-        `?a b. check_partial_col f l live1 flive1 = SOME (a, b)` by metis_tac [check_partial_col_input_monotone] >>
+        qabbrev_tac `lrd = l0` >> qabbrev_tac `lwr = l` >> rpt (qpat_x_assum `Abbrev _` kall_tac) >>
+        fs [case_eq_thms] >> rveq >>
+        `?v. check_partial_col f lwr live flive = SOME v` by metis_tac [check_partial_col_input_monotone] >>
         rw [] >>
-        `is_subset (numset_list_delete l live1) (numset_list_delete l live2)` by metis_tac [numset_list_delete_monotone] >>
-        sg `INJ f (domain (numset_list_delete l live2)) UNIV` THEN1 (
+        `INJ f (domain live) UNIV` by metis_tac [INJ_SUBSET, UNIV_SUBSET] >>
+        `IMAGE f (domain (numset_list_delete lwr live)) = domain (numset_list_delete (MAP f lwr) flive)` by metis_tac [numset_list_delete_IMAGE] >>
+        `IMAGE f (domain (numset_list_delete lwr live')) = domain (numset_list_delete (MAP f lwr) flive')` by metis_tac [numset_list_delete_IMAGE] >>
+        sg `INJ f (domain (numset_list_delete lwr live')) UNIV` THEN1 (
           rw [domain_numset_list_delete] >>
-          `(domain live2 DIFF set l) SUBSET (domain live2)` by fs [SUBSET_DIFF] >>
+          `(domain live' DIFF set lwr) SUBSET (domain live')` by fs [SUBSET_DIFF] >>
           metis_tac [SUBSET_DIFF, INJ_SUBSET, UNIV_SUBSET]
         ) >>
-        sg `IMAGE f (domain (numset_list_delete l live1)) = domain (numset_list_delete (MAP f l) flive1)` THEN1 (
-            `INJ f (domain live1) UNIV` by metis_tac [is_subset_def, INJ_SUBSET, UNIV_SUBSET] >>
-            metis_tac [numset_list_delete_IMAGE]
-        ) >>
-        sg `IMAGE f (domain (numset_list_delete l live2)) = domain (numset_list_delete (MAP f l) flive2)` THEN1 (
-            metis_tac [numset_list_delete_IMAGE]
-        ) >>
-        `?live1' flive1'. check_partial_col f l0 (numset_list_delete l live1)
-        (numset_list_delete (MAP f l) flive1) = SOME (live1', flive1')` by metis_tac [check_partial_col_input_monotone] >>
-        `is_subset live1' live2'` by metis_tac [check_partial_col_output_monotone] >>
-        `IMAGE f (domain live1') = domain flive1'` by metis_tac [check_partial_col_IMAGE] >>
-        rw []
+        `domain (numset_list_delete lwr live) SUBSET domain (numset_list_delete lwr live')` by fs [domain_numset_list_delete, SUBSET_DEF] >>
+        `?live1' flive1'. check_partial_col f lrd (numset_list_delete lwr live) (numset_list_delete (MAP f lwr) flive) = SOME (live1', flive1')` by metis_tac [check_partial_col_input_monotone] >>
+        rw [] >>
+        imp_res_tac check_partial_col_domain >>
+        fs [] >> fs [domain_numset_list_delete, SUBSET_DEF]
     )
 
     (* Set *)
     THEN1 (
         rw [check_clash_tree_def, get_live_tree_def, check_live_tree_def] >>
-        `domain live2' = (set (MAP FST (toAList s))) UNION (domain live2)` by metis_tac [check_partial_col_domain, FST] >>
-        `INJ f (domain live2') UNIV` by metis_tac [check_partial_col_success_INJ] >>
+        imp_res_tac check_partial_col_domain >> fs [] >>
+        imp_res_tac check_partial_col_success_INJ >> rfs [] >>
         `set (MAP FST (toAList s)) = domain s` by rw [EXTENSION, MEM_MAP, EXISTS_PROD, MEM_toAList, domain_lookup] >>
-        `domain live2' = domain s UNION domain live2` by metis_tac [check_partial_col_domain, FST] >>
-        `domain s SUBSET domain live2'` by rw [SUBSET_DEF] >>
+        fs [] >>
+        `domain s SUBSET domain s UNION domain live'` by fs [] >>
         `INJ f (domain s) UNIV` by metis_tac [INJ_SUBSET, UNIV_SUBSET] >>
-        `?live1' flive1'. check_col f s = SOME (live1', flive1')` by metis_tac [check_col_success] >>
-        qexists_tac `live1'` >>
-        qexists_tac `flive1'` >>
-        rw []
-        THEN1 metis_tac [check_col_output]
-        THEN1 fs [check_col_def, is_subset_def]
+        `?livein flivein. check_col f s = SOME (livein, flivein)` by metis_tac [check_col_success] >>
+        rw [] >>
+        fs [check_col_def]
     )
 
     (* Branch *)
     THEN1 (
         rw [check_clash_tree_def, get_live_tree_def, check_live_tree_def] >>
-        fs [check_live_tree_def] >>
-        Cases_on `o'` >> fs [check_live_tree_def] >> TRY (rename1 `toAList cutset`) >>
-        Cases_on `check_live_tree f (get_live_tree ct) live2 flive2` >> fs [] >>
-        Cases_on `x` >> fs [] >>
-        Cases_on `check_live_tree f (get_live_tree ct') live2 flive2` >> fs [] >>
-        Cases_on `x` >> fs [] >>
-        `?live11 flive11. check_clash_tree f ct live1 flive1 = SOME (live11, flive11)` by metis_tac [] >>
-        `?live12 flive12. check_clash_tree f ct' live1 flive1 = SOME (live12, flive12)` by metis_tac [] >>
+        Cases_on `o'` >> fs [check_live_tree_def] >>
+        fs [case_eq_thms] >> rveq >>
+        (* Try to get consistent names *)
+        TRY (
+          qabbrev_tac `cutset = x` >>
+          qabbrev_tac `livemid = livein2'` >> qabbrev_tac `flivemid = flivein2'` >>
+          rpt (qpat_x_assum `Abbrev _` kall_tac)
+        ) >>
+        qabbrev_tac `livein1' = livein1` >> qabbrev_tac `flivein1' = flivein1` >>
+        qabbrev_tac `livein2' = livein2` >> qabbrev_tac `flivein2' = flivein2` >>
+        rpt (qpat_x_assum `Abbrev _` kall_tac) >>
+        `?livein1 flivein1. check_clash_tree f ct live flive = SOME (livein1, flivein1) /\ domain livein1 SUBSET domain livein1'` by metis_tac [] >>
+        `?livein2 flivein2. check_clash_tree f ct' live flive = SOME (livein2, flivein2) /\ domain livein2 SUBSET domain livein2'` by metis_tac [] >>
         rw []
         THEN1 (
-            sg `is_subset live11 q` THEN1 (
-              last_x_assum (qspecl_then [`f`, `live1`, `flive1`, `live2`, `flive2`, `q`, `r`] assume_tac) >>
-              res_tac >>
-              `live1'' = live11` by metis_tac [SOME_11, PAIR_EQ] >>
-              fs []
-            ) >>
-            sg `is_subset live12 q'` THEN1 (
-              first_x_assum (qspecl_then [`f`, `live1`, `flive1`, `live2`, `flive2`, `q'`, `r'`] assume_tac) >>
-              res_tac >>
-              `live1'' = live12` by metis_tac [SOME_11, PAIR_EQ] >>
-              fs []
-            ) >>
-            `!(a : num_set) (b : num_set) (c : num_set). is_subset a b ==> is_subset (difference a c) (difference b c)` by rw [is_subset_def, domain_difference, SUBSET_DEF] >>
-            `is_subset (difference live12 q) (difference q' q)` by rw [] >>
-            `domain r = IMAGE f (domain q) /\ INJ f (domain q) UNIV` by metis_tac [check_live_tree_success] >>
-            `?a b. check_partial_col f (MAP FST (toAList (difference live12 q))) q r = SOME (a, b)` by metis_tac [check_partial_col_list_monotone] >>
-            `INJ f (domain live1) UNIV` by metis_tac [is_subset_def, INJ_SUBSET, UNIV_SUBSET] >>
-            `domain flive12 = IMAGE f (domain live12)` by metis_tac [check_clash_tree_output] >>
-            `INJ f (domain live12) UNIV` by metis_tac [check_clash_tree_output] >>
-            `?a fa. check_partial_col f (MAP FST (toAList (difference q live12))) live12 flive12 = SOME (a, fa)` by metis_tac [check_partial_col_branch_comm] >>
-            `is_subset (difference live11 live12) (difference q live12)` by rw [] >>
-            `?b fb. check_partial_col f (MAP FST (toAList (difference live11 live12))) live12 flive12 = SOME (b, fb)` by metis_tac [check_partial_col_list_monotone] >>
-            `domain flive11 = IMAGE f (domain live11)` by metis_tac [check_clash_tree_output] >>
-            `?c fc. check_partial_col f (MAP FST (toAList (difference live12 live11))) live11 flive11 = SOME (c, fc)` by metis_tac [check_partial_col_branch_comm] >>
-            qexists_tac `c` >>
-            qexists_tac `fc` >>
-            simp [] >>
-            strip_tac
-            THEN1 metis_tac [check_partial_col_IMAGE]
-            THEN1 (
-                `domain c = set (MAP FST (toAList (difference live12 live11))) UNION domain live11` by metis_tac [check_partial_col_domain, FST] >>
-                `domain c = domain live11 UNION domain live12` by metis_tac [branch_domain, check_partial_col_domain, FST] >>
-                `domain live2' = domain q UNION domain q'` by metis_tac [branch_domain, check_partial_col_domain, FST] >>
-                rw [is_subset_def] >>
-                rw [SUBSET_DEF] >>
-                metis_tac [SUBSET_DEF, is_subset_def]
-            )
+            imp_res_tac check_live_tree_success >> rfs [] >>
+            `INJ f (set (MAP FST (toAList (difference livein2' livein1'))) UNION domain livein1') UNIV` by metis_tac [check_partial_col_success_INJ] >>
+            `set (MAP FST (toAList (difference livein2 livein1))) UNION domain livein1 SUBSET set (MAP FST (toAList (difference livein2' livein1'))) UNION domain livein1'` by (REWRITE_TAC [branch_domain] >> fs [SUBSET_DEF]) >>
+            `INJ f (set (MAP FST (toAList (difference livein2 livein1))) UNION domain livein1) UNIV` by metis_tac [INJ_SUBSET, UNIV_SUBSET] >>
+            `INJ f (domain live) UNIV` by metis_tac [INJ_SUBSET, UNIV_SUBSET] >>
+            `domain flivein1 = IMAGE f (domain livein1)` by metis_tac [check_clash_tree_output] >>
+            `?livein flivein. check_partial_col f (MAP FST (toAList (difference livein2 livein1))) livein1 flivein1 = SOME (livein, flivein)` by metis_tac [check_partial_col_success] >>
+            rw [] >>
+            `domain livein = set (MAP FST (toAList (difference livein2 livein1))) UNION domain livein1` by metis_tac [check_partial_col_domain, FST] >>
+            `domain livein' = set (MAP FST (toAList (difference livein2' livein1'))) UNION domain livein1'` by metis_tac [check_partial_col_domain, FST] >>
+            rw []
         )
         THEN1 (
-            Cases_on `check_partial_col f (MAP FST (toAList (difference q' q))) q r` >> fs [] >>
-            Cases_on `x` >> fs [] >>
-            `domain r = IMAGE f (domain q) /\ INJ f (domain q) UNIV` by metis_tac [check_live_tree_success] >>
-            `domain r'' = IMAGE f (domain q'') /\ INJ f (domain q'') UNIV` by metis_tac [check_partial_col_IMAGE, check_partial_col_success_INJ] >>
-            `INJ f (domain live2') UNIV` by metis_tac [check_partial_col_IMAGE, check_partial_col_success_INJ] >>
-            `domain live2' = set (MAP FST (toAList cutset)) UNION domain q''` by metis_tac[check_partial_col_domain, FST] >>
+            `domain flivein1' = IMAGE f (domain livein1') /\ INJ f (domain livein1') UNIV` by metis_tac [check_live_tree_success] >>
+            `domain flivein2' = IMAGE f (domain livein2') /\ INJ f (domain livein2') UNIV` by metis_tac [check_live_tree_success] >>
+            `domain flivemid = IMAGE f (domain livemid) /\ INJ f (domain livemid) UNIV` by metis_tac [check_partial_col_success_INJ, check_partial_col_IMAGE] >>
+            `INJ f (domain livein') UNIV` by metis_tac [check_partial_col_success_INJ] >>
+            `domain livein' = set (MAP FST (toAList cutset)) UNION domain livemid` by metis_tac [check_partial_col_domain, FST] >>
             `set (MAP FST (toAList cutset)) = domain cutset` by rw [EXTENSION, MEM_MAP, EXISTS_PROD, MEM_toAList, domain_lookup] >>
-            `domain cutset SUBSET domain live2'` by rw [SUBSET_DEF] >>
+            `domain cutset SUBSET domain livein'` by fs [] >>
             `INJ f (domain cutset) UNIV` by metis_tac [INJ_SUBSET, UNIV_SUBSET] >>
-            `?live1' flive1'. check_col f cutset = SOME (live1', flive1')` by metis_tac [check_col_success] >>
-            qexists_tac `live1'` >>
-            qexists_tac `flive1'` >>
-            rw []
-            THEN1 metis_tac [check_col_output]
-            THEN1 fs [check_col_def, is_subset_def]
+            `?livein flivein. check_col f cutset = SOME (livein, flivein)` by metis_tac [check_col_success] >>
+            rw [] >>
+            fs [check_col_def]
         )
     )
 
     (* Seq *)
     THEN1 (
         rw [check_clash_tree_def, get_live_tree_def, check_live_tree_def] >>
-        Cases_on `check_live_tree f (get_live_tree ct') live2 flive2` >> fs [] >>
-        Cases_on `x` >> fs [] >>
-        `?t2_out ft2_out. check_clash_tree f ct' live1 flive1 = SOME (t2_out, ft2_out) /\ IMAGE f (domain t2_out) = domain ft2_out /\ is_subset t2_out q` by metis_tac [] >>
+        fs [case_eq_thms] >> rveq >>
+        `?t2_out ft2_out. check_clash_tree f ct' live flive = SOME (t2_out, ft2_out) /\ domain t2_out SUBSET domain livein2` by metis_tac [] >>
+        `INJ f (domain live) UNIV` by metis_tac [INJ_SUBSET, UNIV_SUBSET] >>
+        `IMAGE f (domain t2_out) = domain ft2_out` by metis_tac [check_clash_tree_output] >>
         simp [] >>
-        `IMAGE f (domain q) = domain r` by metis_tac [check_live_tree_success] >>
-        `INJ f (domain q) UNIV` by metis_tac [check_live_tree_success] >>
+        `IMAGE f (domain livein2) = domain flivein2` by metis_tac [check_live_tree_success] >>
+        `INJ f (domain livein2) UNIV` by metis_tac [check_live_tree_success] >>
         metis_tac []
     )
 )
 
 val get_live_tree_correct = Q.store_thm("get_live_tree_correct",
-    `!f live flive ct live' flive'.
+    `!f live flive ct livein flivein.
     IMAGE f (domain live) = domain flive ==>
     INJ f (domain live) UNIV ==>
-    check_live_tree f (get_live_tree ct) live flive = SOME (live', flive') ==>
-    ?live'' flive''. check_clash_tree f ct live flive = SOME (live'', flive'')
+    check_live_tree f (get_live_tree ct) live flive = SOME (livein, flivein) ==>
+    ?livein' flivein'. check_clash_tree f ct live flive = SOME (livein', flivein')
     `,
-    metis_tac [get_live_tree_correct_lemma, is_subset_def, SUBSET_REFL]
+    metis_tac [get_live_tree_correct_lemma, SUBSET_REFL]
 )
 
 val get_live_tree_correct_LN = Q.store_thm("get_live_tree_correct_LN",
-    `!f live flive ct live' flive'.
-    check_live_tree f (get_live_tree ct) LN LN = SOME (live', flive') ==>
-    ?live'' flive''. check_clash_tree f ct LN LN = SOME (live'', flive'')
+    `!f live flive ct livein flivein.
+    check_live_tree f (get_live_tree ct) LN LN = SOME (livein, flivein) ==>
+    ?livein' flivein'. check_clash_tree f ct LN LN = SOME (livein', flivein')
     `,
     rw [get_live_tree_correct]
 )
